\documentclass[11pt,a4paper,ngerman]{article}
\usepackage[bottom=2.5cm,top=2.5cm]{geometry} 
\usepackage{babel}
\usepackage[utf8]{inputenc} 
\usepackage[T1]{fontenc} 
\usepackage{ae} 
\usepackage{amssymb} 
\usepackage{amsmath}
\usepackage{amsthm} 
\usepackage{graphicx}
\usepackage{fancyhdr}
\usepackage{fancyref}
\usepackage{listings}
\usepackage{xcolor}
\usepackage{paralist}

\usepackage[pdftex, bookmarks=false, pdfstartview={FitH}, linkbordercolor=white]{hyperref}
\usepackage{fancyhdr}
\pagestyle{fancy}
\fancyhead[C]{Advanced Functional Programming}
\fancyhead[L]{Exercise sheet 2}
\fancyhead[R]{SoSe 2013}
\fancyfoot{}
\fancyfoot[L]{}
\fancyfoot[C]{\thepage \hspace{1px} of \pageref{LastPage}}
\renewcommand{\footrulewidth}{0.5pt}
\renewcommand{\headrulewidth}{0.5pt}
\setlength{\parindent}{0pt} 
\setlength{\headheight}{0pt}

\date{}
\title{Exercise sheet 2}
\author{Max Wisniewski, Alexander Steen}


%%
%% Enviroments for proofs and lemmas
%%
\newtheorem{lemma}{\bfseries lemma}
\newtheorem{claim}{\bfseries claim}

\lstloadlanguages{Haskell}
\lstset{
  language=Haskell,
  basicstyle=\ttfamily,
  flexiblecolumns=false,
  basewidth={0.5em,0.45em},
  literate={+}{{$+$}}1 {/}{{$/$}}1 {*}{{$*$}}1 {=}{{$=$}}1
           {>}{{$>$}}1 {<}{{$<$}}1 {\\}{{$\lambda$}}1
           {\\\\}{{\char`\\\char`\\}}1
           {->}{{$\rightarrow$}}2 {>=}{{$\geq$}}2 {<-}{{$\leftarrow$}}2
           {<=}{{$\leq$}}2 {=>}{{$\Rightarrow$}}2 
           {\ .}{{$\circ$}}2 {\ .\ }{{$\circ$}}2
           {>>}{{>>}}2 {>>=}{{>>=}}2
           {|}{{$\mid$}}1               
}

\lstnewenvironment{code}
    {\lstset{basicstyle=\footnotesize\ttfamily}%
      \csname lst@SetFirstLabel\endcsname}
    {\csname lst@SaveFirstLabel\endcsname}
\long\def\ignore#1{}

\begin{document}

\renewcommand{\figurename}{Figure}
\maketitle
\thispagestyle{fancy}

\section*{Task 1}
We first prove a lemma that is being used in the induction proof of the task's proposition:
\textbf{Lemma}: \lstinline|f (foldNat' f e n) = foldNat' f (f e) n|.\\
\textbf{Proof} by induction:\\
Base: \texttt{n = O}
    \begin{lstlisting}
      f (foldNat' f e O)
    = {Def.}
      f e
    = {Def. inverse}
      foldNat' f (f e) O
    \end{lstlisting}
Step: \texttt{n} $\rightsquigarrow$ \texttt{S n}
    \begin{lstlisting}
      f (foldNat' f e (S n))
    = {Def.}
      f (foldNat' f (f e) n)
    = {Induction Hyp.}
      foldNat' f (f (f e)) n
    = {Def. inverse}
      foldNat' f (f e) (S n)
    \end{lstlisting}
\mbox{} \hfill $\square$

\textbf{Proposition}: \lstinline|foldNat f e = foldNat' f e|.\\
\textbf{Proof} by induction:\\
Base: \texttt{n = O}
    \begin{lstlisting}
      foldNat f e O
    = {Def.}
      e
    = {Def. inverse}
      foldNat' f e 0
    \end{lstlisting}
Step: \texttt{n} $\rightsquigarrow$ \texttt{S n}
    \begin{lstlisting}
      foldNat f e (S n)
    = {Def.}
      f (foldNat f e n)
    = {Induction Hyp.}
      f (foldNat' f e n)
    = {Lemma}
      foldNat' f (f e) n
    = {Def. inverse}
      foldNat' f e (S n)
    \end{lstlisting} 
\mbox{} \hfill $\square$
\input{ueb2.lhs}

\label{LastPage}

\end{document}
